theories/program_logic/delaywp.v
@@ -1,0 +1,147 @@
+From stdpp Require Import base gmap.
+From iris.algebra Require Import auth gmap excl.
+From iris.proofmode Require Import base tactics classes.
+From iris.base_logic.lib Require Export fancy_updates.
+From shiris.program_logic Require Import delaystate.
+Set Default Proof Using "Type".
+
+(* 
+    What should the definition for wp look like?
+    I want to match on the delay type and for answer apply the post condition.
+    For the think branch I want to apply the wp recursively.
+
+    Before I can get to the delay type I first need to run the state somehow.
+    This is a wishful thinking version of the wp definition.
+*)
+Definition state_wp {Σ} {ST A} (SI: ST -> iProp Σ)
+           (e: state_delay ST A) (Φ: A -> iProp Σ): iProp Σ := ∀ σ,
+  SI σ ==∗
+  match runState e σ with
+       | Answer (Some (σ', x)) => Φ x ∗ SI σ'
+       | Answer None => True
+       | Think e' => True (*▷ state_wp SI e'Φ*)
+  end.
+
+(* The actual definition will need Iris fixpoint for this. Let's try finding that somewhere        
+   Wp is here https://gitlab.mpi-sws.org/iris/iris/-/blob/master/theories/program_logic/weakestpre.v#L27
+   The fixpoint is here: https://gitlab.mpi-sws.org/iris/iris/-/blob/master/theories/program_logic/weakestpre.v#L47
+*)
+
+(* Definition state_wp {Σ} {ST A} (SI: ST -> iProp Σ) *)
+           (* (e: state_delay ST A) (Φ: A -> iProp Σ): iProp Σ := ∀ σ, *)
+  (* SI σ ==∗ *)
+  (* ∃σ', ⌜runState e σ = Some (a, σ') ⌝ ∗ *)
+          (* SI σ' ∗ *)
+          (* Φ a. *)
+(*
+  We run into the same problem here as with the evaluator for state_delay: 
+  We need the state aspect for our state interpretation and our notion of separation.
+  We need to get to the Think constructor to recurse in our wp definition on the sub expression.
+  However once we get to the Think node, although it does contain pre_wired stateful operations they are now
+  completely opaque to us.
+
+  In the evaluator we work around this by having the (co-)recursion only work for the delay monad
+  Then add state on top as an extra layer. Can we write a wp that works just for delay?
+*)
+
+Definition wp_delay_pre {Σ} {A} (go: delay A -d> (A -d> iPropO Σ) -d> iPropO Σ):
+      delay A -d> (A -d> iPropO Σ) -d> iPropO Σ.
+refine(λ e Φ, match e with
+              | Answer x => Φ x
+              | Think e' => ▷ go e' Φ
+              end
+              )%I.
+Defined.
+
+Instance wp_delay_pre_contractive {Σ A}: Contractive (@wp_delay_pre Σ A ).
+Proof.
+  rewrite /wp_delay_pre => n wp wp' Hwp e1 Φ.
+  repeat (f_contractive || f_equiv); apply Hwp.
+Qed.
+ 
+Definition wp_delay {Σ} {A}: delay A -> (A -> iProp Σ)-> iProp Σ := fixpoint wp_delay_pre.
+
+Definition wp {Σ} {ST A} (SI: ST -> iProp Σ) (e: state_delay ST A) (Φ: A -> iProp Σ): iProp Σ.
+refine(∀ σ, 
+    SI σ ==∗
+     wp_delay (runState e σ) (λ (res: option (ST * A)), 
+       match res with   
+       | Some (σ', x) => Φ x ∗ SI σ'
+       | None => True
+       end)
+)%I.
+Defined.
+
+Lemma wp_delay_unfold {Σ A} (e: delay A) (Φ: A -> iProp Σ): wp_delay e Φ ≡ wp_delay_pre wp_delay e Φ.
+Proof.
+  apply (fixpoint_unfold wp_delay_pre).
+Qed.
+
+Lemma wp_delay_return {Σ A}(x: A) (Φ: A -> iProp Σ): Φ x -∗ wp_delay (Answer x) Φ.
+Proof.
+   rewrite wp_delay_unfold.
+   done.
+Qed.
+
+Lemma wp_delay_bind {Σ A B} (f: A -> delay B) (Φ: B -> iProp Σ) (e: delay A): 
+  wp_delay e (λ x, wp_delay (f x) Φ) -∗ wp_delay (e ≫= f) Φ.
+Proof.
+  unfold mbind, mbind_delay.
+  iIntros "H". iLöb as "IH" forall (e).
+  iEval (rewrite wp_delay_unfold).
+  unfold wp_delay_pre.
+  destruct e; simpl.
+  - rewrite wp_delay_unfold /=. rewrite wp_delay_unfold /=.
+    unfold wp_delay_pre. done.
+  - iEval (rewrite wp_delay_unfold /=) in "H".
+    iNext. iApply "IH". done.
+Qed.
+
+Lemma wp_state_return {Σ A ST } {SI: ST -> iProp Σ} (x: A) (Φ: A -> iProp Σ): Φ x -∗ wp SI (mret x) Φ.
+Proof.
+  iIntros "H" (σ) "HSi".
+  simpl.
+  iApply wp_delay_return. by iFrame.
+Qed.
+
+(* 
+  change to delay.
+  proof bind.
+  get load store.
+  iter combinators.
+*)
+Lemma wp_strong_mono {Σ A} (e: delay A) (Φ Ψ: A -> iProp Σ) :
+  wp_delay e Φ -∗ (∀ v, Φ v -∗ Ψ v) -∗ wp_delay e Ψ.
+Proof.
+  iLöb as "IH" forall (e).
+  rewrite wp_delay_unfold.
+  rewrite wp_delay_unfold.
+  iIntros "Hwp H".
+  unfold wp_delay_pre.
+  destruct e; simpl.
+  - iApply ("H" with "Hwp").
+  - iNext. iApply ("IH" $! e with "Hwp H"). 
+Qed.
+
+Locate "|==>".
+Print bupd.
+Lemma wp_state_bind {Σ A B ST} {SI: ST -> iProp Σ} (f: A -> state_delay ST B) (Φ: B -> iProp Σ) (e: state_delay ST A): 
+  wp SI e (λ x, wp SI (f x) Φ) -∗ wp SI (e ≫= f) Φ.
+Proof.
+  iIntros "H" (σ) "HSi". rewrite /mbind /mbind_state_delay /=.
+  iApply wp_delay_bind.
+  iMod ("H" with  "HSi") as "H".
+  iModIntro.
+  iApply (wp_strong_mono with "[H]").
+  - done.
+  - iIntros (v).
+    destruct v.
+    + destruct p. iIntros "(Hwp & HSi)".
+      (* Stuck with an update modality here from wp (state)
+       can we do wp_strong_mono with an update modality?
+       No we can't because wp_delay does not have an update modality in it's definition *)
+      unfold wp. iSpecialize ("Hwp" $! (s) with "HSi").
+
+    +
+
+About fixpoint. 
